Add ArrayTest.sum

platform/tests/ArrayTest.v
@@ -19,14 +19,21 @@ Definition incS := SPEC("arr", "len") reserving 2
   PRE[V] array8 arr (V "arr") * [| V "len" = length arr |] * [| goodSize (length arr) |]
   POST[_] array8 (inc arr) (V "arr").
 
+Definition sum ls := fold_left (fun n b => n ^+ BtoW b) ls $0.
+
+Definition sumS := SPEC("arr", "len") reserving 3
+  Al arr,
+  PRE[V] array8 arr (V "arr") * [| V "len" = length arr |] * [| goodSize (length arr) |]
+  POST[R] array8 arr (V "arr") * [| R = sum arr |].
+
 Definition m := bmodule "array" {{
-  (*bfunction "read"("arr", "pos") [readS]
+  bfunction "read"("arr", "pos") [readS]
     "arr" <-*8 "arr" + "pos";;
     Return "arr"
   end with bfunction "write"("arr", "pos", "val") [writeS]
     "arr" + "pos" *<-8 "val";;
     Return 0
-  end with*) bfunction "inc"("arr", "len", "i", "tmp") [incS]
+  end with bfunction "inc"("arr", "len", "i", "tmp") [incS]
     "i" <- 0;;
 
     [Al arr,
@@ -43,6 +50,21 @@ Definition m := bmodule "array" {{
     };;
 
     Return 0
+  end with bfunction "sum"("arr", "len", "i", "acc", "tmp") [sumS]
+    "i" <- 0;;
+    "acc" <- 0;;
+
+    [Al done, Al rem,
+      PRE[V] array8 (done ++ rem) (V "arr") * [| V "len" = length (done ++ rem) |]
+        * [| goodSize (length (done ++ rem)) |] * [| V "i" = length done |]
+      POST[R] array8 (done ++ rem) (V "arr") * [| R = V "acc" ^+ sum rem |] ]
+    While ("i" < "len") {
+      "tmp" <-*8 "arr" + "i";;
+      "acc" <- "acc" + "tmp";;
+      "i" <- "i" + 1
+    };;
+
+    Return "acc"
   end
 }}.
 
@@ -183,6 +205,104 @@ Qed.
 
 Hint Resolve final_bound.
 
+Lemma reveal_middle' : forall (ls1 ls2 : list B),
+  (length ls1 < length (ls1 ++ ls2))%nat
+  -> exists x, exists ls2', ls2 = x :: ls2'.
+  intros; rewrite app_length in *.
+  assert (length ls2 <> 0) by omega.
+  destruct ls2; simpl in *; intuition eauto.
+Qed.
+
+Lemma reveal_middle : forall (ls1 ls2 : list B) i len,
+  i < len
+  -> i = natToW (length ls1)
+  -> len = natToW (length (ls1 ++ ls2))
+  -> goodSize (length (ls1 ++ ls2))
+  -> exists x, exists ls2', ls2 = x :: ls2'.
+  intros; subst.
+  eapply reveal_middle'.
+  instantiate (1 := ls1).
+  rewrite app_length in *.
+  pre_nomega.
+  rewrite wordToNat_natToWord_idempotent in H.
+  rewrite wordToNat_natToWord_idempotent in H; assumption.
+  Transparent goodSize.
+  red in H2.
+  generalize dependent (Npow2 32); intros.
+  nomega.
+  Opaque goodSize.
+Qed.
+
+Hint Rewrite DepList.pf_list_simpl : sepFormula.
+
+Lemma length_addendum : forall A (x : A) ls,
+  length (ls ++ x :: nil) = length ls + 1.
+  intros; rewrite app_length; auto.
+Qed.
+
+Hint Rewrite length_addendum : sepFormula.
+
+Lemma sum_cons' : forall acc1 bs acc2,
+  fold_left (fun n b => n ^+ BtoW b) bs (acc1 ^+ acc2) = acc1 ^+ fold_left (fun n b => n ^+ BtoW b) bs acc2.
+  induction bs; simpl; intuition idtac.
+  rewrite <- wplus_assoc.
+  apply IHbs.
+Qed.
+
+Lemma sum_cons : forall b bs,
+  sum (b :: bs) = BtoW b ^+ sum bs.
+  unfold sum; simpl.
+  intros.
+  rewrite wplus_comm; apply sum_cons'.
+Qed.
+
+Hint Rewrite sum_cons : sepFormula.
+
+Lemma selN_middle : forall post mid pre,
+  Array8.selN (pre ++ mid :: post) (length pre) = mid.
+  induction pre; simpl; intuition.
+Qed.
+
+Lemma sel_middle : forall i pre mid post,
+  i = natToW (length pre)
+  -> goodSize (length pre)
+  -> Array8.sel (pre ++ mid :: post) i = mid.
+  unfold Array8.sel; intros; subst.
+  autorewrite with N.
+  apply selN_middle.
+Qed.
+
+Hint Rewrite sel_middle using solve [ eauto 1 ] : sepFormula.
+
+Lemma goodSize_split : forall A (ls1 ls2 : list A),
+  goodSize (length (ls1 ++ ls2))
+  -> goodSize (length ls1).
+  intros; rewrite app_length in *; eapply goodSize_weaken; eauto.
+Qed.
+
+Hint Immediate goodSize_split.
+
+Lemma all_done : forall len i A (done rem : list A),
+  len <= i
+  -> len = natToW (length (done ++ rem))
+  -> i = natToW (length done)
+  -> goodSize (length (done ++ rem))
+  -> rem = nil.
+  intros; subst.
+  rewrite app_length in *.
+  pre_nomega.
+  assert (goodSize (length done)); eauto.
+  rewrite wordToNat_natToWord_idempotent in *; eauto.
+  rewrite wordToNat_natToWord_idempotent in *; eauto.
+  destruct rem; simpl in *; auto; omega.
+Qed.
+
+Lemma sum_nil : sum nil = $0.
+  auto.
+Qed.
+
+Hint Rewrite sum_nil : sepFormula.
+
 Ltac useHyp := match goal with
                  | [ H : forall j : nat, _ |- _ ] => rewrite H by omega
                end.
@@ -190,14 +310,34 @@ Ltac useHyp := match goal with
 Ltac finish :=
   match goal with
     | [ |- _ ^+ _ <= _ ] => eauto
+    | [ |- sel _ "len" = natToW (length (?X ++ _))%nat ] => equate X (@nil B); simpl;
+      eauto; reflexivity || words
     | [ |- himp _ (array8 ?A _) (array8 ?B _) ] =>
       replace B with A by eauto using determine_inc; reflexivity
+    | [ H : sel _ "i" = _ |- _ ^+ natToW 1 = natToW (length _ + 1) ] => solve [ rewrite H; descend ]
+    | [ _ : goodSize (length (_ ++ ?X)) |- _ ] => assert (X = nil) by eauto using all_done; subst;
+      autorewrite with sepFormula; words
     | _ => solve [ useHyp; auto ]
     | _ => solve [ rewrite selN_oob; eauto ]
     | [ H : (?N >= ?M)%nat |- _ ] => destruct (eq_nat_dec N M); subst;
       useHyp; auto; rewrite selN_upd_ne; auto
+    | _ => eauto; reflexivity || words
   end.
 
+Ltac t :=
+  try match goal with
+        | [ |- forall stn_st specs, interp _ _ -> interp _ _ ] =>
+          match goal with
+            | [ |- context[LvMem8] ] => post; evaluate auto_ext;
+              match goal with
+                | [ H : goodSize (length (?done ++ _)) |- _ ] =>
+                  let Ho := fresh in
+                    generalize H; intro Ho; eapply reveal_middle in Ho; eauto; destruct Ho as [ mid [ rem ] ]; subst;
+                      exists (done ++ mid :: nil); exists rem
+              end
+          end
+      end; sep_auto; finish.
+
 Theorem ok : moduleOk m.
-  vcgen; abstract (sep_auto; finish).
+  vcgen; abstract t.
 Qed.
